gol_sim_cvScript.sml
@@ -4,17 +4,6 @@ open HolKernel gol_simTheory boolSyntax computeLib cv_transLib
 
 val _ = new_theory "gol_sim_cv";
 
-Definition single_check_def:
-  single_check (x:int) y d delta =
-     case d of
-     | N => (x,y - delta)
-     | S => (x,y + delta)
-     | E => (x + delta,y)
-     | W => (x - delta,y)
-End
-
-val _ = cv_trans single_check_def;
-
 Definition member_def:
   member x [] = F ∧
   member x (y::ys) = if x = y then T else member x ys
@@ -27,53 +16,6 @@ Theorem member_thm:
 Proof
   Induct \\ gvs [member_def]
 QED
-
-Definition check_io_def:
-  check_io area [] (delta:int) = T ∧
-  check_io area (((x,y),d,_)::rest) delta =
-    (check_io area rest delta ∧
-     member (single_check x y d delta) area)
-End
-
-val _ = cv_trans check_io_def;
-
-Theorem check_io_thm:
-  check_io area ins delta ⇔
-  EVERY (λ((x,y),d,r). d = N ⇒ MEM (x,y − delta) area) ins ∧
-  EVERY (λ((x,y),d,r). d = S ⇒ MEM (x,y + delta) area) ins ∧
-  EVERY (λ((x,y),d,r). d = E ⇒ MEM (x + delta,y) area) ins ∧
-  EVERY (λ((x,y),d,r). d = W ⇒ MEM (x − delta,y) area) ins
-Proof
-  Induct_on ‘ins’ \\ gvs [pairTheory.FORALL_PROD,check_io_def,member_thm]
-  \\ gen_tac \\ gen_tac \\ Cases
-  \\ gvs [single_check_def] \\ eq_tac \\ rw [] \\ gvs []
-QED
-
-(*
-
-Theorem simple_checks_eq:
-  simple_checks w h ins outs rows
-  ⇔
-  rectangle w h rows ∧ h ≠ 0 ∧ w ≠ 0 ∧
-  ALL_DISTINCT (MAP FST ins ++ MAP FST outs) ∧
-  EVERY (λ((x,y),r).
-           (x % 2 = 0 ⇎ y % 2 = 0) ∧ -1 ≤ x ∧ -1 ≤ y ∧ x ≤ 2 * &w − 1 ∧
-           y ≤ 2 * &h − 1) (ins ++ outs) ∧
-  let
-     area = make_area w h
-  in
-    ALL_DISTINCT area ∧
-    check_io area ins 1 ∧
-    check_io area outs (-1)
-Proof
-  gvs [simple_checks_def,check_io_thm, GSYM integerTheory.int_sub]
-  \\ gvs [AC CONJ_COMM CONJ_ASSOC]
-QED
-
-val _ = cv_auto_trans simple_checks_eq;
-val _ = cv_auto_trans simulation_ok_def;
-
-*)
 
 val pre = cv_auto_trans_pre blist_gol_rows_def;
 
@@ -96,11 +38,10 @@ Theorem blist_simple_checks_eq:
      area = make_area w h
   in
     ALL_DISTINCT area ∧
-    check_io area ins 1 ∧
-    check_io area outs (-1)
+    EVERY (λ(p,d,r). member (add_pt p (dir_to_xy d)) area) ins ∧
+    EVERY (λ(p,d,r). member (sub_pt p (dir_to_xy d)) area) outs
 Proof
-  gvs [blist_simple_checks_def,check_io_thm, GSYM integerTheory.int_sub]
-  \\ gvs [AC CONJ_COMM CONJ_ASSOC]
+  gvs [blist_simple_checks_def, member_thm]
 QED
 
 val _ = cv_auto_trans blist_simple_checks_eq;
